coq_ssprove/src/Hacspec_Lib.v
@@ -22,8 +22,7 @@ Import List.ListNotations.
 
 (********************************************************)
 (*   Implementation of all Hacspec library functions    *)
-(* for Both types. Should be enough to get state and    *)
-(* both functions working. TODO: transition to packages *)
+(* for Both types.                                      *)
 (********************************************************)
 
 (*** Integers *)
@@ -40,24 +39,61 @@ Open Scope hacspec_scope.
 Open Scope nat_scope.
 Open Scope list_scope.
 
+Equations lift3_both {A B C : ChoiceEquality} L1 L2 I : (A -> B -> C) -> both L1 I A -> both L2 I B -> both (L1 :|: L2) I C :=
+  lift3_both _ _ _ f x y :=
+    {| is_pure := f x y ;
+      is_state := {code temp_x ← x ;; temp_y ← y ;; ret (f (ct_T temp_x) (ct_T temp_y)) } |}.
+Next Obligation.
+  intros.
+  ssprove_valid ; eapply valid_injectLocations ; [ apply fsubsetUl | | apply fsubsetUr | ] ; apply (prog_valid (is_state _)).
+Qed.
+Next Obligation.
+  intros.
+  pattern_both Hb Hf Hg.
+  apply (@r_bind_trans_both A C).
+  subst Hf Hg Hb ; hnf.
+  pattern_both Hb Hf Hg.
+  apply (@r_bind_trans_both B C).
+  subst Hf Hg Hb ; hnf.
+  rewrite !ct_T_id.
+  apply r_ret. easy.
+Qed.
+Global Transparent lift3_both.
+
+Equations lift2_both {A B : ChoiceEquality} {L} {I} : (A -> B) -> both L I A -> both L I B :=
+  lift2_both f x :=
+    {| is_pure := f x ;
+      is_state := {code temp_x ← x ;; ret (f (ct_T temp_x)) } |}.
+Next Obligation.
+  intros.
+  pattern_both Hb Hf Hg.
+  apply (@r_bind_trans_both A B).
+  subst Hf Hg Hb ; hnf.
+  rewrite !ct_T_id.
+  apply r_ret. easy.
+Qed.
+Global Transparent lift2_both.
+
 Section IntType.
-Definition int_modi {WS : wsize} : @int WS -> @int WS -> both0 (@int WS) := fun x y => lift_to_both (int_modi x y).
-Definition int_add {WS : wsize} : @int WS -> @int WS -> both0 (@int WS) := fun x y => lift_to_both (int_add x y).
-Definition int_sub {WS : wsize} : @int WS -> @int WS -> both0 (@int WS) := fun x y => lift_to_both (int_sub x y).
-Definition int_opp {WS : wsize} : @int WS -> both0 (@int WS) := fun x => lift_to_both (int_opp x).
-Definition int_mul {WS : wsize} : @int WS -> @int WS -> both0 (@int WS) := fun x y => lift_to_both (int_mul x y).
-Definition int_div {WS : wsize} : @int WS -> @int WS -> both0 (@int WS) := fun x y => lift_to_both (int_div x y).
-Definition int_mod {WS : wsize} : @int WS -> @int WS -> both0 (@int WS) := fun x y => lift_to_both (int_mod x y).
-Definition int_xor {WS : wsize} : @int WS -> @int WS -> both0 (@int WS) := fun x y => lift_to_both (int_xor x y).
-Definition int_and {WS : wsize} : @int WS -> @int WS -> both0 (@int WS) := fun x y => lift_to_both (int_and x y).
-Definition int_or {WS : wsize} : @int WS -> @int WS -> both0 (@int WS) := fun x y => lift_to_both (int_or x y).
-Definition int_not {WS : wsize} : @int WS -> both0 (@int WS) := fun x => lift_to_both (int_not x).
+  Definition int_modi {WS : wsize} {L1 L2} {I} := @lift3_both _ _ (@int WS) L1 L2 I int_modi.
+  Definition int_add {WS : wsize} {L1 L2} {I} := @lift3_both _ _ (@int WS) L1 L2 I int_add.
+  Definition int_sub {WS : wsize} {L1 L2} {I} := @lift3_both _ _ (@int WS) L1 L2 I int_sub.
+  Definition int_opp {WS : wsize} {L} {I} := @lift2_both _ (@int WS) L I int_opp.
+  Definition int_mul {WS : wsize} {L1 L2} {I} := @lift3_both _ _ (@int WS) L1 L2 I int_mul.
+  Definition int_div {WS : wsize} {L1 L2} {I} := @lift3_both _ _ (@int WS) L1 L2 I int_div.
+  Definition int_mod {WS : wsize} {L1 L2} {I} := @lift3_both _ _ (@int WS) L1 L2 I int_mod.
+  Definition int_xor {WS : wsize} {L1 L2} {I} := @lift3_both _ _ (@int WS) L1 L2 I  int_xor.
+  Definition int_and {WS : wsize} {L1 L2} {I} := @lift3_both _ _ (@int WS) L1 L2 I int_and.
+  Definition int_or  {WS : wsize} {L1 L2} {I} := @lift3_both _ _ (@int WS) L1 L2 I int_or.
+  Definition int_not {WS : wsize} {L} {I} := @lift2_both _ (@int WS) L I int_not.
+
+  Program Definition cast_int {WS1 WS2 : wsize} {L I} := @lift2_both (@int WS1) (@int WS2) L I (fun n => repr (unsigned n)).
 End IntType.
 
 Definition secret : forall {WS : wsize},  (T (@int WS)) -> both0 (@int WS) :=
   fun {WS} x => lift_to_both (secret x).
 
-Infix "%%" := int_modi (at level 40, left associativity) : Z_scope.
+Infix ".%%" := int_modi (at level 40, left associativity) : Z_scope.
 Infix ".+" := int_add (at level 77) : hacspec_scope.
 Infix ".-" := int_sub (at level 77) : hacspec_scope.
 Notation "-" := int_opp (at level 77) : hacspec_scope.
@@ -68,19 +104,6 @@ Infix ".^" := int_xor (at level 77) : hacspec_scope.
 Infix ".&" := int_and (at level 77) : hacspec_scope.
 Infix ".|" := int_or (at level 77) : hacspec_scope.
 Notation "'not'" := int_not (at level 77) : hacspec_scope.
-
-Section IntTypeBoth.
-Definition int_modi_both {WS : wsize} {L I} : both L I (@int WS) -> both L I (@int WS) -> both L I (@int WS) := fun x y => lift_to_both (int_modi x y).
-Definition int_add_both {WS : wsize} {L I} : both L I (@int WS) -> both L I (@int WS) -> both L I (@int WS) := fun x y => lift_to_both (int_add x y).
-Definition int_sub_both {WS : wsize} {L I} : both L I (@int WS) -> both L I (@int WS) -> both L I (@int WS) := fun x y => lift_to_both (int_sub x y).
-Definition int_opp_both {WS : wsize} {L I} : both L I (@int WS) -> both L I (@int WS) := fun x => lift_to_both (int_opp x).
-Definition int_mul_both {WS : wsize} {L I} : both L I (@int WS) -> both L I (@int WS) -> both L I (@int WS) := fun x y => lift_to_both (int_mul x y).
-Definition int_div_both {WS : wsize} {L I} : both L I (@int WS) -> both L I (@int WS) -> both L I (@int WS) := fun x y => lift_to_both (int_div x y).
-Definition int_mod_both {WS : wsize} {L I} : both L I (@int WS) -> both L I (@int WS) -> both L I (@int WS) := fun x y => lift_to_both (int_mod x y).
-Definition int_xor_both {WS : wsize} {L I} : both L I (@int WS) -> both L I (@int WS) -> both L I (@int WS) := fun x y => lift_to_both (int_xor x y).
-Definition int_and_both {WS : wsize} {L I} : both L I (@int WS) -> both L I (@int WS) -> both L I (@int WS) := fun x y => lift_to_both (int_and x y).
-Definition int_or_both {WS : wsize}  {L I}: both L I (@int WS) -> both L I (@int WS) -> both L I (@int WS) := fun x y => lift_to_both (int_or x y).
-End IntTypeBoth.
 
 Section Uint.
   Definition uint8_declassify (n : int8) : both0 int8 :=
@@ -125,7 +148,6 @@ Section Uint.
   Definition int128_classify (n : int128) : both0 int128 :=
     lift_to_both (int128_classify n).
 
-
   (* CompCert integers' signedness is only interpreted through 'signed' and 'unsigned',
    and not in the representation. Therefore, uints are just names for their respective ints.
    *)
@@ -135,7 +157,6 @@ Section Uint.
   Definition declassify_u32_from_uint32 (n : uint32) : both0 uint32 :=
     lift_to_both (declassify_u32_from_uint32 n).
 
-  (* Should maybe use size of s instead? *)
   Definition uint8_rotate_left (u: int8) (s: int8) : both0 int8 := lift_to_both (uint8_rotate_left u s).
 
   Definition uint8_rotate_right (u: int8) (s: int8) : both0 (int8) := lift_to_both0 (uint8_rotate_right u s).
@@ -165,20 +186,38 @@ lift_to_both0 (uint128_rotate_left u s).
 lift_to_both0 (uint128_rotate_right u s).
 
 
-  (* should use size u instead of u? *)
   Definition usize_shift_right_ (u: uint_size) (s: int32) : both0 (uint_size) :=
     lift_to_both (u usize_shift_right s).
 
-  (* should use size u instead of u? *)
-  Definition usize_shift_left_ (u: uint_size) (s: int32) : both0 (uint_size) :=
-    lift_to_both (u usize_shift_left s).
+  Program Definition usize_shift_left_ (u: both0 uint_size) (s: both0 int32) : both0 (uint_size) :=
+    {|
+      is_pure := (is_pure u) usize_shift_left (is_pure s) ;
+      is_state :=
+      {code
+         temp_u ← is_state u ;;
+         temp_s ← is_state s ;;
+         ret (T_ct (temp_u usize_shift_left temp_s))
+      }
+    |}.
+  Next Obligation.
+    intros.
+    pattern_both Hb Hf Hg.
+    apply (@r_bind_trans_both (uint_size) (uint_size)).
+    subst Hf Hg Hb ; hnf.
+    pattern_both Hb Hf Hg.
+    apply (@r_bind_trans_both (int32)).
+    subst Hf Hg Hb ; hnf.
+    apply r_ret.
+    easy.
+  Qed.
 
   (**** Operations *)
 
-  Definition shift_left_ `{WS : wsize} (i : @int WS) (j : uint_size) : both0 (@int WS) := lift_to_both (@shift_left_ WS i j).
+  Program Definition shift_left_ `{WS : wsize} {L1 L2} {I} :=
+    @lift3_both _ _ _ L1 L2 I (@shift_left_ WS).
 
-  Definition shift_right_ `{WS : wsize} (i : @int WS) (j : uint_size) : both0 (@int WS):=
-    lift_to_both (@shift_right_ WS i j).
+  Program Definition shift_right_ `{WS : wsize} {L1 L2} {I} :=
+    @lift3_both _ _ _ L1 L2 I (@shift_right_ WS).
 
 End Uint.
 
@@ -203,7 +242,7 @@ Section Loops.
     | O => ret cur
     | S n' =>
         cur' ← f i cur ;;
-        Si ← i .+ one ;;
+        Si ← (lift_to_both0 i) .+ (lift_to_both0 one) ;;
         foldi_ n' Si f (ct_T cur')
     end.
 
@@ -259,7 +298,7 @@ Section Loops.
       {L I}
       (f : T uint_size -> T acc -> code L I (ct acc))
       (cur : T acc),
-      (cur' ← f i cur ;; Si ← i .+ one ;; foldi_ fuel Si f (ct_T cur')) = foldi_ (S fuel) i f cur.
+      (cur' ← f i cur ;; Si ← (lift_to_both0 i) .+ (lift_to_both0 one) ;; foldi_ fuel Si f (ct_T cur')) = foldi_ (S fuel) i f cur.
   Proof. reflexivity. Qed.
 
   Lemma foldi__nat_move_S :
@@ -378,7 +417,7 @@ Section Loops.
       (cur : T acc),
       (0 <= Z.of_nat fuel <= @wmax_unsigned U32)%Z ->
       (cur' ← foldi_ fuel i f cur ;;
-       fuel_add_i ← (repr (Z.of_nat fuel)) .+ i ;;
+       fuel_add_i ← (lift_to_both0 (repr (Z.of_nat fuel))) .+ (lift_to_both0 i) ;;
        f fuel_add_i (ct_T cur')
       ) = foldi_ (S (fuel)) i f cur.
   Proof.
@@ -403,18 +442,17 @@ Section Loops.
       unfold int_add at 1 3.
       unfold lift_to_both, is_state at 1 3.
       unfold prog, lift_to_code.
-      do 2 rewrite bind_rewrite.
+      do 2 setoid_rewrite bind_rewrite.
 
       specialize (IHfuel (Hacspec_Lib_Pre.int_add i one) L I f (ct_T x)).
 
 
 
-      replace ((repr (Z.of_nat (S fuel)) .+ i))
-        with (repr (Z.of_nat fuel) .+ Hacspec_Lib_Pre.int_add i one).
+      replace (Hacspec_Lib_Pre.int_add (repr (Z.of_nat (S fuel))) _)
+        with (Hacspec_Lib_Pre.int_add (repr (Z.of_nat fuel)) (Hacspec_Lib_Pre.int_add i one)).
       2 : {
         unfold int_add.
         unfold Hacspec_Lib_Pre.int_add.
-        f_equal.
         rewrite <- addwC.
         rewrite <- addwA.
         rewrite addwC.
@@ -466,7 +504,7 @@ Section Loops.
   (* folds and natural number folds compute the same thing *)
   Lemma foldi_to_foldi_nat :
     forall {acc: ChoiceEquality}
-      (lo: T uint_size) (* {lo <= hi} *)
+      (lo: T uint_size)
       (hi: T uint_size) (* {lo <= hi} *)
       {L I}
       (f: (T uint_size) -> T acc -> code L I (ct acc)) (* {i < hi} *)
@@ -521,12 +559,13 @@ Section Loops.
 
           unfold int_add.
 
-          replace (@Hacspec_Lib_Pre.int_add U32 (@repr U32 (Z.of_nat (S n))) (@repr U32 (Z.of_nat lo_n))) with (@repr U32 (Z.of_nat (Init.Nat.add (S n) lo_n))). reflexivity.
+          setoid_rewrite bind_rewrite.
+          replace (@Hacspec_Lib_Pre.int_add U32 _ _) with (@repr U32 (Z.of_nat (Init.Nat.add (S n) lo_n))). reflexivity.
 
           apply word_ext.
 
-          replace (urepr (repr (Z.of_nat (S n)))) with (@unsigned U32 (repr (Z.of_nat (S n)))) by reflexivity.
-          replace (urepr (repr (Z.of_nat lo_n))) with (@unsigned U32 (repr (Z.of_nat lo_n))) by reflexivity.
+          replace (urepr _) with (@unsigned U32 (repr (Z.of_nat (S n)))) by reflexivity.
+          replace (urepr _) with (@unsigned U32 (repr (Z.of_nat lo_n))) by reflexivity.
           do 2 rewrite unsigned_repr_alt by lia.
           rewrite Nat2Z.inj_add.
           reflexivity.
@@ -534,7 +573,7 @@ Section Loops.
 
   Lemma foldi_nat_to_foldi :
     forall {acc: ChoiceEquality}
-      (lo: nat) (* {lo <= hi} *)
+      (lo: nat)
       (hi: nat) (* {lo <= hi} *)
       {L I}
       (f: nat -> T acc -> code L I (ct acc)) (* {i < hi} *)
@@ -920,14 +959,16 @@ Definition seq_update_slice
   lift_to_both (seq_update_slice out start_out input start_in len).
 
 Definition seq_concat
-  {a : ChoiceEquality}
+           {a : ChoiceEquality}
+           `{Default a}
   (s1 :(T (seq a)))
   (s2: (T (seq a)))
   : both0 ((seq a)) :=
    lift_to_both (seq_concat s1 s2).
 
 Definition seq_push
-  {a : ChoiceEquality}
+           {a : ChoiceEquality}
+           `{Default a}
   (s1 :(T (seq a)))
   (s2: (T (a)))
   : both0 ((seq a)) :=
@@ -987,8 +1028,6 @@ Definition seq_set_chunk
 Definition seq_num_exact_chunks {a} (l : (T (seq a))) (chunk_size : (T (uint_size))) : (both0 uint_size) :=
   lift_to_both (seq_num_exact_chunks l chunk_size).
 
-
-(* Until #84 is fixed this returns an empty sequence if not enough *)
 Definition seq_get_exact_chunk {a : ChoiceEquality} `{Default (T (a))} (l : (T (seq a))) (chunk_size chunk_num: (T (uint_size))) :
   both0 ((seq a)) :=
   lift_to_both (seq_get_exact_chunk l chunk_size chunk_num).
@@ -1002,7 +1041,7 @@ Definition seq_get_remainder_chunk {a : ChoiceEquality} `{Default (T (a))} (l : 
 Definition seq_xor_ {WS} (x y : seq (@int WS)) : both0 (seq (@int WS)) :=
   lift_to_both (seq_xor_ x y).
 
-Definition seq_truncate {a} (x : seq a) (n : nat) : both0 (seq a) :=
+Definition seq_truncate {a : ChoiceEquality} `{Default a} (x : seq a) (n : nat) : both0 (seq a) :=
   lift_to_both (seq_truncate x n).
 
 End Seqs.
@@ -1033,9 +1072,9 @@ Section Arrays.
     lift_to_both (update_sub v i n sub).
 
   Definition array_from_list
-             (A: ChoiceEquality)
+             {A: ChoiceEquality}
              (l: list (T A))
-    : both0 (nseq A (length l)) := lift_to_both (array_from_list A l).
+    : both0 (nseq A (length l)) := lift_to_both (array_from_list l).
 
   Definition array_from_seq   {a: ChoiceEquality}
              `{Default (T a)}
@@ -1044,7 +1083,7 @@ Section Arrays.
     : both0 (nseq a out_len) :=
     lift_to_both (array_from_seq out_len input).
 
-  Definition array_to_seq {A : ChoiceEquality} {n} (f : nseq A n) : both0 (seq _) :=
+  Definition array_to_seq {A : ChoiceEquality} `{H_default : Default A} {n} (f : nseq A n) : both0 (seq _) :=
     @lift_to_both (seq A) _ _ (array_to_seq f).
 
   Definition array_from_slice
@@ -1242,11 +1281,11 @@ Definition nat_mod_get_bit {p} (a : nat_mod p) n : both0 (nat_mod p) :=
 
 Definition array_declassify_eq {A l} (x : nseq A l) (y : nseq A l) : both0 bool_ChoiceEquality := lift_to_both0 (array_declassify_eq x y).
 Definition array_to_le_uint32s {A l} (x : nseq A l) : both0 (seq uint32) := lift_to_both0 (array_to_le_uint32s x).
-Definition array_to_be_uint32s {l} (x : nseq uint8 l) : both0 (seq uint32) := lift_to_both0 (array_to_be_uint32s x).  (* (l/4) *)
-Definition array_to_le_uint64s {A l} (x : nseq A l) : both0 (seq uint64) := lift_to_both0 (array_to_le_uint64s x).  (* (l/8) *)
-Definition array_to_be_uint64s {l} (x : nseq uint8 l) : both0 (seq uint64) := lift_to_both0 (array_to_be_uint64s x).  (* (l/8) *)
-Definition array_to_le_uint128s {A l} (x : nseq A l) : both0 (seq uint128) := lift_to_both0 (array_to_le_uint128s x).  (* (l/16) *)
-Definition array_to_be_uint128s {l} (x : nseq uint8 l) : both0 (seq uint128) := lift_to_both0 (array_to_be_uint128s x).  (* (l/16) *)
+Definition array_to_be_uint32s {l} (x : nseq uint8 l) : both0 (seq uint32) := lift_to_both0 (array_to_be_uint32s x).
+Definition array_to_le_uint64s {A l} (x : nseq A l) : both0 (seq uint64) := lift_to_both0 (array_to_le_uint64s x).
+Definition array_to_be_uint64s {l} (x : nseq uint8 l) : both0 (seq uint64) := lift_to_both0 (array_to_be_uint64s x).
+Definition array_to_le_uint128s {A l} (x : nseq A l) : both0 (seq uint128) := lift_to_both0 (array_to_le_uint128s x).
+Definition array_to_be_uint128s {l} (x : nseq uint8 l) : both0 (seq uint128) := lift_to_both0 (array_to_be_uint128s x).
 Definition array_to_le_bytes {A l} (x : nseq A l) : both0 (seq uint8) := lift_to_both0 (array_to_le_bytes x).
 Definition array_to_be_bytes {A l} (x : nseq A l) : both0 (seq uint8) := lift_to_both0 (array_to_be_bytes x).
 Definition nat_mod_from_byte_seq_le {A n} (x : seq A) : both0 (nat_mod n) := lift_to_both0 (nat_mod_from_byte_seq_le x).
@@ -1406,27 +1445,6 @@ Next Obligation.
   - inversion_clear H1. now do 2 rewrite eqb_refl.
 Defined.
 
-(*** Be Bytes *)
-
-
-Fixpoint nat_be_range_at_position (k : nat) (z : Z) (n : Z) : list bool :=
-  match k with
-  | O => []
-  | S k' => Z.testbit z (n + k') :: nat_be_range_at_position k' z n
-  end.
-
-Fixpoint nat_be_range_to_position_ (z : list bool) (val : Z) : Z :=
-  match z with
-  | [] => val
-  | x :: xs => nat_be_range_to_position_ xs ((if x then 2 ^ List.length xs else 0) + val)
-  end.
-
-Definition nat_be_range_to_position (k : nat) (z : list bool) (n : Z) : Z :=
-  (nat_be_range_to_position_ z 0 * 2^(k * n)).
-
-Definition nat_be_range (k : nat) (z : Z) (n : nat) : Z :=
-  nat_be_range_to_position_ (nat_be_range_at_position k z (n * k)) 0. (* * 2^(k * n) *)
-
 End TodoSection2.
 
 
@@ -1582,17 +1600,17 @@ Definition CE_loc_to_loc :=
 Notation "'CE_loc_to_CE'" := (@projT1 ChoiceEquality (fun _ => nat)).
 Coercion CE_loc_to_loc : ChoiceEqualityLocation >-> Location.
 
-Definition let_mut_code  {L : {fset Location}} {I} {B : ChoiceEquality}
+Equations let_mut_code  {L : {fset Location}} {I} {B : ChoiceEquality}
            (x_loc : ChoiceEqualityLocation)
            `{H_in: is_true (ssrbool.in_mem (CE_loc_to_loc x_loc) (ssrbool.mem L))}
            (x : code L I (CE_loc_to_CE x_loc)) (f : (CE_loc_to_CE x_loc) -> code L I B) : code L I B :=
-  (let (A, n) as s
-   return (is_true (ssrbool.in_mem (let '(k; n) := s in (ct k; n)) (ssrbool.mem L)) ->
-           code L I (CE_loc_to_CE s) -> (CE_loc_to_CE s -> code L I B) -> code L I B) :=
-     x_loc in
-   fun (_ : is_true (ssrbool.in_mem (ct A; n) (ssrbool.mem L)))
-     (x : code L I (CE_loc_to_CE (A; n))) (f : CE_loc_to_CE (A; n) -> code L I B) =>
-   {code y ← x ;; #put (ct A; n) := y ;; f (ct_T y) }) H_in x f.
+  let_mut_code (A; n) x f :=
+    {code
+       y ← x ;;
+       #put (ct A; n) := y ;;
+       temp ← get (ct A; n) ;;
+       f (ct_T temp) }.
+Global Transparent let_mut_code.
 
 Notation "'letmc' x 'loc(' ℓ ')' ':=' y 'in' f" :=
   (let_mut_code ℓ (H_in := _) y (fun x => f x))
@@ -1619,14 +1637,13 @@ Next Obligation.
 
   apply rpre_hypothesis_rule.
   intros ? ? [[] []]. subst.
-  eapply rpre_weaken_rule with (pre := true_precond).
 
+  apply better_r_put_get_lhs.
   apply better_r_put_lhs.
 
-  rewrite ct_T_id.
+  rewrite !ct_T_id.
   eapply rpre_weaken_rule with (pre := true_precond).
   apply f.
-  reflexivity.
   reflexivity.
 Qed.
 
@@ -2012,6 +2029,7 @@ Fixpoint for_loop_return_ (ℓ : list ChoiceEqualityLocation) (vars : list (∑ 
     cbn in r.
     apply r.
 Defined.
+
 Definition for_loop_return (ℓ : list ChoiceEqualityLocation) : raw_code (list_types (seq.map (fun '(x ; y) => x) ℓ)) := for_loop_return_ ℓ [].
 
 Definition for_loop_locations
@@ -2048,7 +2066,6 @@ Proof.
   intros.
   apply H0.
 Qed.
-
 
 Ltac pattern_foldi_both Hx Hf Hg :=
   match goal with
@@ -2089,7 +2106,7 @@ Ltac progress_step_code :=
   || (match_bind_trans_both)
   || match goal with
     | [ |- context [ ⊢ ⦃ _ ⦄ (#put ?l := ?x ;; (getr ?l ?a)) ≈ _ ⦃ _ ⦄ ]] =>
-        apply better_r_put_get
+        apply better_r_put_get_lhs
     end
   ||
   match goal with
@@ -2170,25 +2187,21 @@ Ltac ssprove_valid_step :=
      (
        cbv zeta
        || unfold prog
-       || (repeat match goal with | [ |- context[ @T_ct (prod_ChoiceEquality ?ceA ?ceB) (?a , ?b) ] ] => rewrite @T_ct_prod_propegate end) (* expensive *)
-       || (match goal with | [ |- context[ @bind ?A ?B (ret ?x) ?f ]] => rewrite bind_rewrite end) (* expensive *)
-       (* if statement *)
+       || (repeat match goal with | [ |- context[ @T_ct (prod_ChoiceEquality ?ceA ?ceB) (?a , ?b) ] ] => rewrite @T_ct_prod_propegate end)
+       || (match goal with | [ |- context[ @bind ?A ?B (ret ?x) ?f ]] => rewrite bind_rewrite end)
        || match goal with
          | [ |- context[match ?x with | true => _ | false => _ end] ] =>
              destruct x
          end
-       (* destruct tt *)
        || match goal with
          | [ |- context[match ?x with | tt => _ end] ] =>
              destruct x
          end
-       (* match expression ? *)
        || match goal with
          | [ |- context[match ?x with | inl _ => _ | inr _ => _ end] ] =>
              destruct x
          end
-       || (match goal with | [ |- context[bind (bind ?v ?k1) ?k2] ] => rewrite bind_assoc end) (* expensive *)
-       (* let statement / array update *)
+       || (match goal with | [ |- context[bind (bind ?v ?k1) ?k2] ] => rewrite bind_assoc end)
        || (apply valid_bind ; [apply valid_scheme ; try rewrite <- fset.fset0E ; apply prog_valid | intros])
        || (apply valid_bind ; [valid_program | intros])
        || (apply valid_bind ; [repeat ssprove_valid_step | intros])
@@ -2201,15 +2214,13 @@ Ltac ssprove_valid_step :=
        || match goal with
          | [ |- context [ getr _ _ ] ] => (apply valid_getr ; [ ssprove_valid_location | intros])
          end
-       (* ret statement *)
        || apply valid_ret
-       (* for looop statement *)
        || (match goal with
           | [ |- context [ValidCode (fset ?ys) _ (@prog _ _ _ (@foldi _ ?lo ?hi (fset ?xs) _ ?f ?v))] ] =>
               eapply (valid_subset_fset xs ys) ; [ | apply valid_foldi_pre ]
               ; loc_incl_compute
           end)
-       || (hnf in * ; destruct_choice_type_prod) (* expensive *)
+       || (hnf in * ; destruct_choice_type_prod)
   )).
 
 Theorem length_merge_sort_pop : forall {A} leb (l1 : list (list A)) (l2 : list A),
@@ -2358,15 +2369,16 @@ Proof.
   apply code_ext. unfold prog.
   unfold let_mut_both, is_state at 1.
   unfold lift_scope. unfold is_state at 1.
-  unfold let_mut_code.
+  rewrite let_mut_code_equation_1.
   unfold prog.
   unfold lift_code_scope.
   rewrite H_var_eq.
   apply f_equal.
   apply functional_extensionality. intros.
   apply f_equal.
-  rewrite H_fun_eq.
-  reflexivity.
+  apply f_equal.
+  apply functional_extensionality. intros.
+  now rewrite H_fun_eq.
 Qed.
 
 Ltac letbm_eq_code :=
@@ -2377,71 +2389,55 @@ Ltac letbm_eq_code :=
 Ltac f_equal_fun_ext :=
   repeat (apply f_equal ; try (apply Coq.Logic.FunctionalExtensionality.functional_extensionality ; intros)).
 
-Definition seq_link { L1 L2 : {fset Location} } {I M E} (p1 : package L1 M E) (p2 : package L2 I M) : package (L1 :|: L2) I E :=
-  {| pack := pkg_composition.link p1 p2 ;
-    pack_valid := pkg_composition.valid_link _ _ _ _ _ _ _
-                                             (pack_valid p1)
-                                             (pack_valid p2) |}.
+Definition u32_word_t := nseq uint8 4.
+Definition u128_word_t := nseq uint8 16.
 
-Program Definition seq_link_both { L1 L2 : {fset Location} } {I} {M : InterfaceCE} {E} (p1 : both_package L1 (IfToCEIf M) E) (p2 : both_package L2 I M) : both_package (L1 :|: L2) I E :=
-  {|
-    pack_pure o H X := @pack_pure _ _ _ p1 o H X ;
-    pack_state := seq_link p1 p2 ;
-    pack_eq_proof_statement := _
-  |}.
-Next Obligation.
+Lemma letbm_ret_r :
+  forall {A : choice.Choice.type} {B : ChoiceEquality}
+    (r₁ : raw_code A) (pre : precond)
+    (post : postcond (choice.Choice.sort A) (choice.Choice.sort B))
+    (ℓ : ChoiceEqualityLocation)
+    (L : {fset Location})
+    (I : Interface)
+    v (f : _ -> both L I B) (H_in : is_true (ssrbool.in_mem (CE_loc_to_loc ℓ) (ssrbool.mem L))),
+    ⊢ ⦃ (set_rhs (@existT choice_type (fun _ : choice_type => nat) (ct (projT1 ℓ)) (projT2 ℓ)) v pre) ⦄ r₁ ≈ f v ⦃ post ⦄ ->
+    ⊢ ⦃ pre ⦄ r₁ ≈ let_mut_both ℓ (H_in := H_in) (lift_to_both (ct_T v)) f ⦃ post ⦄.
+Proof.
   intros.
-  apply p1.
   cbn.
-Admitted.
+  unfold let_mut_code.
+  unfold lift_to_code.
+  unfold Hacspec_Lib.let_mut_both_obligation_1.
+  cbn.
+  destruct ℓ.
+  cbn.
+  apply better_r_put_get_rhs.
+  apply better_r, r_put_rhs.
+  rewrite !T_ct_id.
+  apply H.
+Qed.
 
-Definition par_link { L1 L2 : {fset Location} }  { I1 I2 E1 E2} (p1 : package L1 I1 E1) (p2 : package L2 I2 E2) (_ : pkg_composition.Parable p1 p2) : package (L1 :|: L2) (I1 :|: I2) (E1 :|: E2) :=
-  {|
-    pack := pkg_composition.par p1 p2 ;
-    pack_valid := pkg_composition.valid_par _ _ _ _ _ _ _ _ _ (pack_valid p1) (pack_valid p2) |}.
-
-Program Definition par_link_both { L1 L2 : {fset Location} }  { I1 I2 E1 E2} (p1 : both_package L1 I1 E1) (p2 : both_package L2 I2 E2) (_ : pkg_composition.Parable p1 p2) : both_package (L1 :|: L2) (I1 :|: I2) (E1 ++ E2) :=
-  {|
-    pack_pure o H X := _ ;
-    pack_state :=
-    {|
-      pack := pkg_composition.par p1 p2 ;
-      pack_valid := pkg_composition.valid_par _ _ _ _ _ _ _ _ _ (pack_valid p1) (pack_valid p2)
-    |}
-  |}.
-Next Obligation.
+Lemma letbm_ret_l :
+  forall {A : ChoiceEquality} {B : choice.Choice.type}
+    (r₀ : raw_code A)
+    (r₁ : raw_code B) (pre : precond)
+    (post : postcond (choice.Choice.sort A) (choice.Choice.sort B))
+    (ℓ : ChoiceEqualityLocation)
+    (L : {fset Location})
+    (I : Interface)
+    v (f : _ -> both L I A) (H_in : is_true (ssrbool.in_mem (CE_loc_to_loc ℓ) (ssrbool.mem L))),
+    ⊢ ⦃ (set_lhs (@existT choice_type (fun _ : choice_type => nat) (ct (projT1 ℓ)) (projT2 ℓ)) v pre) ⦄ f v ≈ r₁ ⦃ post ⦄ ->
+    ⊢ ⦃ pre ⦄ let_mut_both ℓ (H_in := H_in) (lift_to_both (ct_T v)) f ≈ r₁ ⦃ post ⦄.
+Proof.
   intros.
-  apply in_app_or in H.
-  admit.
-Admitted.
-Next Obligation.
-  intros.
-  unfold IfToCEIf.
-  generalize dependent p1.
-  induction E1.
-  - cbn.
-    rewrite <- fset0E.
-    rewrite fset0U.
-    reflexivity.
-  - cbn.
-    rewrite fset_cons.
-    fold (IfToCEIf E1).
-    rewrite <- fsetUA.
-    intros.
-Admitted.
-Next Obligation.
-Admitted.
-
-Notation "'link_rest(' a ')'" :=
-  a : hacspec_scope.
-Notation "'link_rest(' a , b ')'" :=
-  (par_link a b _) : hacspec_scope.
-Notation "'link_rest(' a , b , .. , c ')'" :=
-  (par_link .. ( par_link a b _ ) .. c _) : hacspec_scope.
-
-Notation "'link_rest_both(' a ')'" :=
-  a : hacspec_scope.
-Notation "'link_rest_both(' a , b ')'" :=
-  (par_link_both a b _) : hacspec_scope.
-Notation "'link_rest_both(' a , b , .. , c ')'" :=
-  (par_link_both .. ( par_link_both a b _ ) .. c _) : hacspec_scope.
+  cbn.
+  unfold let_mut_code.
+  unfold lift_to_code.
+  unfold Hacspec_Lib.let_mut_both_obligation_1.
+  cbn.
+  destruct ℓ.
+  apply better_r_put_get_lhs.
+  apply better_r_put_lhs.
+  rewrite !T_ct_id.
+  apply H.
+Qed.
