coq_ssprove/_vc/Hacspec_Sha256.v
@@ -1,0 +1,563 @@
+(** This file was automatically generated using Hacspec **)
+Set Warnings "-notation-overridden,-ambiguous-paths".
+From Crypt Require Import choice_type Package Prelude.
+Import PackageNotation.
+From extructures Require Import ord fset.
+From mathcomp.word Require Import ssrZ word.
+From Jasmin Require Import word.
+
+From Coq Require Import ZArith.
+Import List.ListNotations.
+Open Scope list_scope.
+Open Scope Z_scope.
+Open Scope bool_scope.
+
+Require Import ChoiceEquality.
+Require Import LocationUtility.
+Require Import Hacspec_Lib_Comparable.
+Require Import Hacspec_Lib_Pre.
+Require Import Hacspec_Lib.
+
+Open Scope hacspec_scope.
+
+Obligation Tactic := try timeout 8 solve_ssprove_obligations.
+
+
+Definition block_size_v : uint_size :=
+  usize 64.
+
+Definition len_size_v : uint_size :=
+  usize 8.
+
+Definition k_size_v : uint_size :=
+  usize 64.
+
+Definition hash_size_v : uint_size :=
+  ((usize 256) ./ (usize 8)).
+
+Definition block_t := nseq (uint8) (block_size_v).
+
+Definition op_table_type_t := nseq (uint_size) (usize 12).
+
+Definition sha256_digest_t := nseq (uint8) (hash_size_v).
+
+Definition round_constants_table_t := nseq (uint32) (k_size_v).
+
+Definition hash_t := nseq (uint32) (usize 8).
+
+
+Notation "'ch_inp'" :=(
+  uint32 '× uint32 '× uint32 : choice_type) (in custom pack_type at level 2).
+Notation "'ch_inp'" :=(
+  uint32 '× uint32 '× uint32 : ChoiceEquality) (at level 2).
+Notation "'ch_out'" :=(uint32 : choice_type) (in custom pack_type at level 2).
+Notation "'ch_out'" :=(uint32 : ChoiceEquality) (at level 2).
+Definition CH : nat :=
+  835.
+Program Definition ch (x_832 : uint32) (y_833 : uint32) (z_834 : uint32)
+  : both (fset.fset0) [interface] (uint32) :=
+  ((lift_scope (H_loc_incl := _) (H_opsig_incl := _) (((
+            lift_to_both0 x_832) .& (lift_to_both0 y_833)) .^ ((not (
+              lift_to_both0 x_832)) .& (lift_to_both0 z_834)))
+      ) : both (fset.fset0) [interface] (uint32)).
+Fail Next Obligation.
+
+
+Notation "'maj_inp'" :=(
+  uint32 '× uint32 '× uint32 : choice_type) (in custom pack_type at level 2).
+Notation "'maj_inp'" :=(
+  uint32 '× uint32 '× uint32 : ChoiceEquality) (at level 2).
+Notation "'maj_out'" :=(uint32 : choice_type) (in custom pack_type at level 2).
+Notation "'maj_out'" :=(uint32 : ChoiceEquality) (at level 2).
+Definition MAJ : nat :=
+  839.
+Program Definition maj (x_836 : uint32) (y_837 : uint32) (z_838 : uint32)
+  : both (fset.fset0) [interface] (uint32) :=
+  ((lift_scope (H_loc_incl := _) (H_opsig_incl := _) (((
+            lift_to_both0 x_836) .& (lift_to_both0 y_837)) .^ (((
+              lift_to_both0 x_836) .& (lift_to_both0 z_838)) .^ ((
+              lift_to_both0 y_837) .& (lift_to_both0 z_838))))
+      ) : both (fset.fset0) [interface] (uint32)).
+Fail Next Obligation.
+
+Definition op_table_v : op_table_type_t :=
+  @array_from_list uint_size [
+    (usize 2) : uint_size;
+    (usize 13) : uint_size;
+    (usize 22) : uint_size;
+    (usize 6) : uint_size;
+    (usize 11) : uint_size;
+    (usize 25) : uint_size;
+    (usize 7) : uint_size;
+    (usize 18) : uint_size;
+    (usize 3) : uint_size;
+    (usize 17) : uint_size;
+    (usize 19) : uint_size;
+    (usize 10) : uint_size
+  ].
+
+Definition k_table_v : round_constants_table_t :=
+  @array_from_list uint32 [
+    (secret (@repr U32 1116352408)) : uint32;
+    (secret (@repr U32 1899447441)) : uint32;
+    (secret (@repr U32 3049323471)) : uint32;
+    (secret (@repr U32 3921009573)) : uint32;
+    (secret (@repr U32 961987163)) : uint32;
+    (secret (@repr U32 1508970993)) : uint32;
+    (secret (@repr U32 2453635748)) : uint32;
+    (secret (@repr U32 2870763221)) : uint32;
+    (secret (@repr U32 3624381080)) : uint32;
+    (secret (@repr U32 310598401)) : uint32;
+    (secret (@repr U32 607225278)) : uint32;
+    (secret (@repr U32 1426881987)) : uint32;
+    (secret (@repr U32 1925078388)) : uint32;
+    (secret (@repr U32 2162078206)) : uint32;
+    (secret (@repr U32 2614888103)) : uint32;
+    (secret (@repr U32 3248222580)) : uint32;
+    (secret (@repr U32 3835390401)) : uint32;
+    (secret (@repr U32 4022224774)) : uint32;
+    (secret (@repr U32 264347078)) : uint32;
+    (secret (@repr U32 604807628)) : uint32;
+    (secret (@repr U32 770255983)) : uint32;
+    (secret (@repr U32 1249150122)) : uint32;
+    (secret (@repr U32 1555081692)) : uint32;
+    (secret (@repr U32 1996064986)) : uint32;
+    (secret (@repr U32 2554220882)) : uint32;
+    (secret (@repr U32 2821834349)) : uint32;
+    (secret (@repr U32 2952996808)) : uint32;
+    (secret (@repr U32 3210313671)) : uint32;
+    (secret (@repr U32 3336571891)) : uint32;
+    (secret (@repr U32 3584528711)) : uint32;
+    (secret (@repr U32 113926993)) : uint32;
+    (secret (@repr U32 338241895)) : uint32;
+    (secret (@repr U32 666307205)) : uint32;
+    (secret (@repr U32 773529912)) : uint32;
+    (secret (@repr U32 1294757372)) : uint32;
+    (secret (@repr U32 1396182291)) : uint32;
+    (secret (@repr U32 1695183700)) : uint32;
+    (secret (@repr U32 1986661051)) : uint32;
+    (secret (@repr U32 2177026350)) : uint32;
+    (secret (@repr U32 2456956037)) : uint32;
+    (secret (@repr U32 2730485921)) : uint32;
+    (secret (@repr U32 2820302411)) : uint32;
+    (secret (@repr U32 3259730800)) : uint32;
+    (secret (@repr U32 3345764771)) : uint32;
+    (secret (@repr U32 3516065817)) : uint32;
+    (secret (@repr U32 3600352804)) : uint32;
+    (secret (@repr U32 4094571909)) : uint32;
+    (secret (@repr U32 275423344)) : uint32;
+    (secret (@repr U32 430227734)) : uint32;
+    (secret (@repr U32 506948616)) : uint32;
+    (secret (@repr U32 659060556)) : uint32;
+    (secret (@repr U32 883997877)) : uint32;
+    (secret (@repr U32 958139571)) : uint32;
+    (secret (@repr U32 1322822218)) : uint32;
+    (secret (@repr U32 1537002063)) : uint32;
+    (secret (@repr U32 1747873779)) : uint32;
+    (secret (@repr U32 1955562222)) : uint32;
+    (secret (@repr U32 2024104815)) : uint32;
+    (secret (@repr U32 2227730452)) : uint32;
+    (secret (@repr U32 2361852424)) : uint32;
+    (secret (@repr U32 2428436474)) : uint32;
+    (secret (@repr U32 2756734187)) : uint32;
+    (secret (@repr U32 3204031479)) : uint32;
+    (secret (@repr U32 3329325298)) : uint32
+  ].
+
+Definition hash_init_v : hash_t :=
+  @array_from_list uint32 [
+    (secret (@repr U32 1779033703)) : uint32;
+    (secret (@repr U32 3144134277)) : uint32;
+    (secret (@repr U32 1013904242)) : uint32;
+    (secret (@repr U32 2773480762)) : uint32;
+    (secret (@repr U32 1359893119)) : uint32;
+    (secret (@repr U32 2600822924)) : uint32;
+    (secret (@repr U32 528734635)) : uint32;
+    (secret (@repr U32 1541459225)) : uint32
+  ].
+
+Definition tmp_840_loc : ChoiceEqualityLocation :=
+  (uint32 ; 841%nat).
+Notation "'sigma_inp'" :=(
+  uint32 '× uint_size '× uint_size : choice_type) (in custom pack_type at level 2).
+Notation "'sigma_inp'" :=(
+  uint32 '× uint_size '× uint_size : ChoiceEquality) (at level 2).
+Notation "'sigma_out'" :=(
+  uint32 : choice_type) (in custom pack_type at level 2).
+Notation "'sigma_out'" :=(uint32 : ChoiceEquality) (at level 2).
+Definition SIGMA : nat :=
+  845.
+Program Definition sigma (x_842 : uint32) (i_843 : uint_size) (
+    op_844 : uint_size)
+  : both (CEfset ([tmp_840_loc])) [interface] (uint32) :=
+  ((letbm tmp_840 : uint32 loc( tmp_840_loc ) :=
+        uint32_rotate_right (lift_to_both0 x_842) (array_index (op_table_v) (((
+                lift_to_both0 (usize 3)) .* (lift_to_both0 i_843)) .+ (
+              lift_to_both0 (usize 2)))) in
+      letb '(tmp_840) :=
+        if (lift_to_both0 op_844) =.? (lift_to_both0 (
+            usize 0)) :bool_ChoiceEquality
+        then lift_scope (L1 := CEfset ([tmp_840_loc])) (L2 := CEfset (
+            [tmp_840_loc])) (I1 := [interface]) (
+          I2 := [interface]) (H_loc_incl := _) (H_opsig_incl := _) (
+          letbm tmp_840 loc( tmp_840_loc ) :=
+            (lift_to_both0 x_842) shift_right (array_index (op_table_v) (((
+                    lift_to_both0 (usize 3)) .* (lift_to_both0 i_843)) .+ (
+                  lift_to_both0 (usize 2)))) in
+          lift_scope (H_loc_incl := _) (H_opsig_incl := _) (
+            lift_to_both0 tmp_840)
+          )
+        else lift_scope (H_loc_incl := _) (H_opsig_incl := _) (
+          lift_to_both0 tmp_840)
+         in
+      lift_scope (H_loc_incl := _) (H_opsig_incl := _) (((uint32_rotate_right (
+              lift_to_both0 x_842) (array_index (op_table_v) ((lift_to_both0 (
+                    usize 3)) .* (lift_to_both0 i_843)))) .^ (
+            uint32_rotate_right (lift_to_both0 x_842) (array_index (
+                op_table_v) (((lift_to_both0 (usize 3)) .* (
+                    lift_to_both0 i_843)) .+ (lift_to_both0 (usize 1)))))) .^ (
+          lift_to_both0 tmp_840))
+      ) : both (CEfset ([tmp_840_loc])) [interface] (uint32)).
+Fail Next Obligation.
+
+Definition s_846_loc : ChoiceEqualityLocation :=
+  (round_constants_table_t ; 847%nat).
+Notation "'schedule_inp'" :=(
+  block_t : choice_type) (in custom pack_type at level 2).
+Notation "'schedule_inp'" :=(block_t : ChoiceEquality) (at level 2).
+Notation "'schedule_out'" :=(
+  round_constants_table_t : choice_type) (in custom pack_type at level 2).
+Notation "'schedule_out'" :=(
+  round_constants_table_t : ChoiceEquality) (at level 2).
+Definition SCHEDULE : nat :=
+  857.
+Program Definition schedule (block_848 : block_t)
+  : both (CEfset ([tmp_840_loc ; s_846_loc])) [interface] (
+    round_constants_table_t) :=
+  ((letb b_849 : seq uint32 := array_to_be_uint32s (lift_to_both0 block_848) in
+      letbm s_846 : round_constants_table_t loc( s_846_loc ) :=
+        array_new_ (default : uint32) (k_size_v) in
+      letb s_846 :=
+        foldi_both' (lift_to_both0 (usize 0)) (lift_to_both0 k_size_v) s_846 (
+            L := (CEfset ([tmp_840_loc ; s_846_loc]))) (I := [interface]) (
+            fun i_850 s_846 =>
+            letb '(s_846) :=
+              if (lift_to_both0 i_850) <.? (lift_to_both0 (
+                  usize 16)) :bool_ChoiceEquality
+              then lift_scope (L1 := CEfset ([s_846_loc])) (L2 := CEfset (
+                  [tmp_840_loc ; s_846_loc])) (I1 := [interface]) (
+                I2 := [interface]) (H_loc_incl := _) (H_opsig_incl := _) (
+                letb s_846 : round_constants_table_t :=
+                  array_upd s_846 (lift_to_both0 i_850) (is_pure (seq_index (
+                        b_849) (lift_to_both0 i_850))) in
+                lift_scope (H_loc_incl := _) (H_opsig_incl := _) (
+                  lift_to_both0 s_846)
+                )
+              else  lift_scope (L1 := CEfset ([tmp_840_loc ; s_846_loc])) (
+                L2 := CEfset ([tmp_840_loc ; s_846_loc])) (I1 := [interface]) (
+                I2 := [interface]) (H_loc_incl := _) (H_opsig_incl := _) (
+                letb t16_851 : uint32 :=
+                  array_index (s_846) ((lift_to_both0 i_850) .- (lift_to_both0 (
+                        usize 16))) in
+                letb t15_852 : uint32 :=
+                  array_index (s_846) ((lift_to_both0 i_850) .- (lift_to_both0 (
+                        usize 15))) in
+                letb t7_853 : uint32 :=
+                  array_index (s_846) ((lift_to_both0 i_850) .- (lift_to_both0 (
+                        usize 7))) in
+                letb t2_854 : uint32 :=
+                  array_index (s_846) ((lift_to_both0 i_850) .- (lift_to_both0 (
+                        usize 2))) in
+                letb s1_855 : uint32 :=
+                  sigma (lift_to_both0 t2_854) (lift_to_both0 (usize 3)) (
+                    lift_to_both0 (usize 0)) in
+                letb s0_856 : uint32 :=
+                  sigma (lift_to_both0 t15_852) (lift_to_both0 (usize 2)) (
+                    lift_to_both0 (usize 0)) in
+                letb s_846 : round_constants_table_t :=
+                  array_upd s_846 (lift_to_both0 i_850) (is_pure ((((
+                            lift_to_both0 s1_855) .+ (
+                            lift_to_both0 t7_853)) .+ (
+                          lift_to_both0 s0_856)) .+ (lift_to_both0 t16_851))) in
+                lift_scope (H_loc_incl := _) (H_opsig_incl := _) (
+                  lift_to_both0 s_846)
+                ) in
+            lift_scope (H_loc_incl := _) (H_opsig_incl := _) (
+              lift_to_both0 s_846)
+            ) in
+      lift_scope (H_loc_incl := _) (H_opsig_incl := _) (lift_to_both0 s_846)
+      ) : both (CEfset ([tmp_840_loc ; s_846_loc])) [interface] (
+      round_constants_table_t)).
+Fail Next Obligation.
+
+Definition h_858_loc : ChoiceEqualityLocation :=
+  (hash_t ; 859%nat).
+Notation "'shuffle_inp'" :=(
+  round_constants_table_t '× hash_t : choice_type) (in custom pack_type at level 2).
+Notation "'shuffle_inp'" :=(
+  round_constants_table_t '× hash_t : ChoiceEquality) (at level 2).
+Notation "'shuffle_out'" :=(
+  hash_t : choice_type) (in custom pack_type at level 2).
+Notation "'shuffle_out'" :=(hash_t : ChoiceEquality) (at level 2).
+Definition SHUFFLE : nat :=
+  873.
+Program Definition shuffle (ws_870 : round_constants_table_t) (
+    hashi_860 : hash_t)
+  : both (CEfset ([tmp_840_loc ; h_858_loc])) [interface] (hash_t) :=
+  ((letbm h_858 : hash_t loc( h_858_loc ) := lift_to_both0 hashi_860 in
+      letb h_858 :=
+        foldi_both' (lift_to_both0 (usize 0)) (lift_to_both0 k_size_v) h_858 (
+            L := (CEfset ([tmp_840_loc ; h_858_loc]))) (I := [interface]) (
+            fun i_861 h_858 =>
+            letb a0_862 : uint32 :=
+              array_index (h_858) (lift_to_both0 (usize 0)) in
+            letb b0_863 : uint32 :=
+              array_index (h_858) (lift_to_both0 (usize 1)) in
+            letb c0_864 : uint32 :=
+              array_index (h_858) (lift_to_both0 (usize 2)) in
+            letb d0_865 : uint32 :=
+              array_index (h_858) (lift_to_both0 (usize 3)) in
+            letb e0_866 : uint32 :=
+              array_index (h_858) (lift_to_both0 (usize 4)) in
+            letb f0_867 : uint32 :=
+              array_index (h_858) (lift_to_both0 (usize 5)) in
+            letb g0_868 : uint32 :=
+              array_index (h_858) (lift_to_both0 (usize 6)) in
+            letb h0_869 : uint32 :=
+              array_index (h_858) (lift_to_both0 (usize 7)) in
+            letb t1_871 : uint32 :=
+              ((((lift_to_both0 h0_869) .+ (sigma (lift_to_both0 e0_866) (
+                        lift_to_both0 (usize 1)) (lift_to_both0 (
+                          usize 1)))) .+ (ch (lift_to_both0 e0_866) (
+                      lift_to_both0 f0_867) (lift_to_both0 g0_868))) .+ (
+                  array_index (k_table_v) (lift_to_both0 i_861))) .+ (
+                array_index (ws_870) (lift_to_both0 i_861)) in
+            letb t2_872 : uint32 :=
+              (sigma (lift_to_both0 a0_862) (lift_to_both0 (usize 0)) (
+                  lift_to_both0 (usize 1))) .+ (maj (lift_to_both0 a0_862) (
+                  lift_to_both0 b0_863) (lift_to_both0 c0_864)) in
+            letb h_858 : hash_t :=
+              array_upd h_858 (lift_to_both0 (usize 0)) (is_pure ((
+                    lift_to_both0 t1_871) .+ (lift_to_both0 t2_872))) in
+            letb h_858 : hash_t :=
+              array_upd h_858 (lift_to_both0 (usize 1)) (is_pure (
+                  lift_to_both0 a0_862)) in
+            letb h_858 : hash_t :=
+              array_upd h_858 (lift_to_both0 (usize 2)) (is_pure (
+                  lift_to_both0 b0_863)) in
+            letb h_858 : hash_t :=
+              array_upd h_858 (lift_to_both0 (usize 3)) (is_pure (
+                  lift_to_both0 c0_864)) in
+            letb h_858 : hash_t :=
+              array_upd h_858 (lift_to_both0 (usize 4)) (is_pure ((
+                    lift_to_both0 d0_865) .+ (lift_to_both0 t1_871))) in
+            letb h_858 : hash_t :=
+              array_upd h_858 (lift_to_both0 (usize 5)) (is_pure (
+                  lift_to_both0 e0_866)) in
+            letb h_858 : hash_t :=
+              array_upd h_858 (lift_to_both0 (usize 6)) (is_pure (
+                  lift_to_both0 f0_867)) in
+            letb h_858 : hash_t :=
+              array_upd h_858 (lift_to_both0 (usize 7)) (is_pure (
+                  lift_to_both0 g0_868)) in
+            lift_scope (H_loc_incl := _) (H_opsig_incl := _) (
+              lift_to_both0 h_858)
+            ) in
+      lift_scope (H_loc_incl := _) (H_opsig_incl := _) (lift_to_both0 h_858)
+      ) : both (CEfset ([tmp_840_loc ; h_858_loc])) [interface] (hash_t)).
+Fail Next Obligation.
+
+Definition h_874_loc : ChoiceEqualityLocation :=
+  (hash_t ; 875%nat).
+Notation "'compress_inp'" :=(
+  block_t '× hash_t : choice_type) (in custom pack_type at level 2).
+Notation "'compress_inp'" :=(block_t '× hash_t : ChoiceEquality) (at level 2).
+Notation "'compress_out'" :=(
+  hash_t : choice_type) (in custom pack_type at level 2).
+Notation "'compress_out'" :=(hash_t : ChoiceEquality) (at level 2).
+Definition COMPRESS : nat :=
+  880.
+Program Definition compress (block_876 : block_t) (h_in_878 : hash_t)
+  : both (CEfset (
+      [tmp_840_loc ; s_846_loc ; h_858_loc ; h_874_loc])) [interface] (
+    hash_t) :=
+  ((letb s_877 : round_constants_table_t :=
+        schedule (lift_to_both0 block_876) in
+      letbm h_874 : hash_t loc( h_874_loc ) :=
+        shuffle (lift_to_both0 s_877) (lift_to_both0 h_in_878) in
+      letb h_874 :=
+        foldi_both' (lift_to_both0 (usize 0)) (lift_to_both0 (usize 8)) h_874 (
+            L := (CEfset ([tmp_840_loc ; s_846_loc ; h_858_loc ; h_874_loc]))) (
+            I := [interface]) (fun i_879 h_874 =>
+            letb h_874 : hash_t :=
+              array_upd h_874 (lift_to_both0 i_879) (is_pure ((array_index (
+                      h_874) (lift_to_both0 i_879)) .+ (array_index (h_in_878) (
+                      lift_to_both0 i_879)))) in
+            lift_scope (H_loc_incl := _) (H_opsig_incl := _) (
+              lift_to_both0 h_874)
+            ) in
+      lift_scope (H_loc_incl := _) (H_opsig_incl := _) (lift_to_both0 h_874)
+      ) : both (CEfset (
+        [tmp_840_loc ; s_846_loc ; h_858_loc ; h_874_loc])) [interface] (
+      hash_t)).
+Fail Next Obligation.
+
+Definition h_881_loc : ChoiceEqualityLocation :=
+  (hash_t ; 885%nat).
+Definition pad_block_884_loc : ChoiceEqualityLocation :=
+  (block_t ; 886%nat).
+Definition last_block_882_loc : ChoiceEqualityLocation :=
+  (block_t ; 887%nat).
+Definition last_block_len_883_loc : ChoiceEqualityLocation :=
+  (uint_size ; 888%nat).
+Notation "'hash_inp'" :=(
+  byte_seq : choice_type) (in custom pack_type at level 2).
+Notation "'hash_inp'" :=(byte_seq : ChoiceEquality) (at level 2).
+Notation "'hash_out'" :=(
+  sha256_digest_t : choice_type) (in custom pack_type at level 2).
+Notation "'hash_out'" :=(sha256_digest_t : ChoiceEquality) (at level 2).
+Definition HASH : nat :=
+  895.
+Program Definition hash (msg_889 : byte_seq)
+  : both (CEfset (
+      [tmp_840_loc ; s_846_loc ; h_858_loc ; h_874_loc ; h_881_loc ; last_block_882_loc ; last_block_len_883_loc ; pad_block_884_loc])) [interface] (
+    sha256_digest_t) :=
+  ((letbm h_881 : hash_t loc( h_881_loc ) := lift_to_both0 hash_init_v in
+      letbm last_block_882 : block_t loc( last_block_882_loc ) :=
+        array_new_ (default : uint8) (block_size_v) in
+      letbm last_block_len_883 : uint_size loc( last_block_len_883_loc ) :=
+        lift_to_both0 (usize 0) in
+      letb '(h_881, last_block_882, last_block_len_883) :=
+        foldi_both' (lift_to_both0 (usize 0)) (seq_num_chunks (
+              lift_to_both0 msg_889) (lift_to_both0 block_size_v)) prod_ce(
+            h_881,
+            last_block_882,
+            last_block_len_883
+          ) (L := (CEfset (
+                [tmp_840_loc ; s_846_loc ; h_858_loc ; h_874_loc ; h_881_loc ; last_block_882_loc ; last_block_len_883_loc ; pad_block_884_loc]))) (
+            I := [interface]) (fun i_890 '(
+              h_881,
+              last_block_882,
+              last_block_len_883
+            ) =>
+            letb '(block_len_891, block_892) : (uint_size '× seq uint8) :=
+              seq_get_chunk (lift_to_both0 msg_889) (
+                lift_to_both0 block_size_v) (lift_to_both0 i_890) in
+            letb '(h_881, last_block_882, last_block_len_883) :=
+              if (lift_to_both0 block_len_891) <.? (
+                lift_to_both0 block_size_v) :bool_ChoiceEquality
+              then lift_scope (L1 := CEfset (
+                  [h_881_loc ; last_block_882_loc ; last_block_len_883_loc])) (
+                L2 := CEfset (
+                  [tmp_840_loc ; s_846_loc ; h_858_loc ; h_874_loc ; h_881_loc ; last_block_882_loc ; last_block_len_883_loc])) (
+                I1 := [interface]) (
+                I2 := [interface]) (H_loc_incl := _) (H_opsig_incl := _) (
+                letbm last_block_882 loc( last_block_882_loc ) :=
+                  array_update_start (array_new_ (default : uint8) (
+                      block_size_v)) (lift_to_both0 block_892) in
+                letbm last_block_len_883 loc( last_block_len_883_loc ) :=
+                  lift_to_both0 block_len_891 in
+                lift_scope (H_loc_incl := _) (H_opsig_incl := _) (prod_b(
+                    lift_to_both0 h_881,
+                    lift_to_both0 last_block_882,
+                    lift_to_both0 last_block_len_883
+                  ))
+                )
+              else  lift_scope (L1 := CEfset (
+                  [tmp_840_loc ; s_846_loc ; h_858_loc ; h_874_loc ; h_881_loc ; last_block_882_loc ; last_block_len_883_loc])) (
+                L2 := CEfset (
+                  [tmp_840_loc ; s_846_loc ; h_858_loc ; h_874_loc ; h_881_loc ; last_block_882_loc ; last_block_len_883_loc])) (
+                I1 := [interface]) (
+                I2 := [interface]) (H_loc_incl := _) (H_opsig_incl := _) (
+                letb compress_input_893 : block_t :=
+                  array_from_seq (block_size_v) (lift_to_both0 block_892) in
+                letbm h_881 loc( h_881_loc ) :=
+                  compress (lift_to_both0 compress_input_893) (
+                    lift_to_both0 h_881) in
+                lift_scope (H_loc_incl := _) (H_opsig_incl := _) (prod_b(
+                    lift_to_both0 h_881,
+                    lift_to_both0 last_block_882,
+                    lift_to_both0 last_block_len_883
+                  ))
+                ) in
+            lift_scope (H_loc_incl := _) (H_opsig_incl := _) (prod_b(
+                lift_to_both0 h_881,
+                lift_to_both0 last_block_882,
+                lift_to_both0 last_block_len_883
+              ))
+            ) in
+      letb last_block_882 : block_t :=
+        array_upd last_block_882 (lift_to_both0 last_block_len_883) (is_pure (
+            secret (lift_to_both0 (@repr U8 128)))) in
+      letb len_bist_894 : uint64 :=
+        secret (pub_u64 (is_pure ((seq_len (lift_to_both0 msg_889)) .* (
+                lift_to_both0 (usize 8))))) in
+      letb '(h_881, last_block_882) :=
+        if (lift_to_both0 last_block_len_883) <.? ((
+            lift_to_both0 block_size_v) .- (
+            lift_to_both0 len_size_v)) :bool_ChoiceEquality
+        then lift_scope (L1 := CEfset (
+            [tmp_840_loc ; s_846_loc ; h_858_loc ; h_874_loc ; h_881_loc ; last_block_882_loc ; last_block_len_883_loc])) (
+          L2 := CEfset (
+            [tmp_840_loc ; s_846_loc ; h_858_loc ; h_874_loc ; h_881_loc ; last_block_882_loc ; last_block_len_883_loc ; pad_block_884_loc])) (
+          I1 := [interface]) (
+          I2 := [interface]) (H_loc_incl := _) (H_opsig_incl := _) (
+          letbm last_block_882 loc( last_block_882_loc ) :=
+            array_update (lift_to_both0 last_block_882) ((
+                lift_to_both0 block_size_v) .- (lift_to_both0 len_size_v)) (
+              array_to_seq (uint64_to_be_bytes (lift_to_both0 len_bist_894))) in
+          letbm h_881 loc( h_881_loc ) :=
+            compress (lift_to_both0 last_block_882) (lift_to_both0 h_881) in
+          lift_scope (H_loc_incl := _) (H_opsig_incl := _) (prod_b(
+              lift_to_both0 h_881,
+              lift_to_both0 last_block_882
+            ))
+          )
+        else  lift_scope (L1 := CEfset (
+            [tmp_840_loc ; s_846_loc ; h_858_loc ; h_874_loc ; h_881_loc ; last_block_882_loc ; last_block_len_883_loc ; pad_block_884_loc])) (
+          L2 := CEfset (
+            [tmp_840_loc ; s_846_loc ; h_858_loc ; h_874_loc ; h_881_loc ; last_block_882_loc ; last_block_len_883_loc ; pad_block_884_loc])) (
+          I1 := [interface]) (
+          I2 := [interface]) (H_loc_incl := _) (H_opsig_incl := _) (
+          letbm pad_block_884 : block_t loc( pad_block_884_loc ) :=
+            array_new_ (default : uint8) (block_size_v) in
+          letbm pad_block_884 loc( pad_block_884_loc ) :=
+            array_update (lift_to_both0 pad_block_884) ((
+                lift_to_both0 block_size_v) .- (lift_to_both0 len_size_v)) (
+              array_to_seq (uint64_to_be_bytes (lift_to_both0 len_bist_894))) in
+          letbm h_881 loc( h_881_loc ) :=
+            compress (lift_to_both0 last_block_882) (lift_to_both0 h_881) in
+          letbm h_881 loc( h_881_loc ) :=
+            compress (lift_to_both0 pad_block_884) (lift_to_both0 h_881) in
+          lift_scope (H_loc_incl := _) (H_opsig_incl := _) (prod_b(
+              lift_to_both0 h_881,
+              lift_to_both0 last_block_882
+            ))
+          ) in
+      lift_scope (H_loc_incl := _) (H_opsig_incl := _) (array_from_seq (
+          hash_size_v) (array_to_be_bytes (lift_to_both0 h_881)))
+      ) : both (CEfset (
+        [tmp_840_loc ; s_846_loc ; h_858_loc ; h_874_loc ; h_881_loc ; last_block_882_loc ; last_block_len_883_loc ; pad_block_884_loc])) [interface] (
+      sha256_digest_t)).
+Fail Next Obligation.
+
+
+Notation "'sha256_inp'" :=(
+  byte_seq : choice_type) (in custom pack_type at level 2).
+Notation "'sha256_inp'" :=(byte_seq : ChoiceEquality) (at level 2).
+Notation "'sha256_out'" :=(
+  sha256_digest_t : choice_type) (in custom pack_type at level 2).
+Notation "'sha256_out'" :=(sha256_digest_t : ChoiceEquality) (at level 2).
+Definition SHA256 : nat :=
+  897.
+Program Definition sha256 (msg_896 : byte_seq)
+  : both (CEfset (
+      [tmp_840_loc ; s_846_loc ; h_858_loc ; h_874_loc ; h_881_loc ; last_block_882_loc ; last_block_len_883_loc ; pad_block_884_loc])) [interface] (
+    sha256_digest_t) :=
+  ((lift_scope (H_loc_incl := _) (H_opsig_incl := _) (hash (
+          lift_to_both0 msg_896))
+      ) : both (CEfset (
+        [tmp_840_loc ; s_846_loc ; h_858_loc ; h_874_loc ; h_881_loc ; last_block_882_loc ; last_block_len_883_loc ; pad_block_884_loc])) [interface] (
+      sha256_digest_t)).
+Fail Next Obligation.
+
